specs/lemmas/Spec.P256.Lemmas.fst
@@ -7,10 +7,13 @@ module M = Lib.NatMod
 
 #set-options "--z3rlimit 50 --ifuel 0 --fuel 0"
 
-let prime_lemma () = admit()
+let prime_lemma c = admit()
 
-let lemma_aff_is_point_at_inf p =
-  prime_lemma ();
+let lemma_exp_prime p x = admit()
+let lemma_exp_inv_prime p x y = admit()
+
+let lemma_aff_is_point_at_inf #c p =
+  prime_lemma c;
   let (px, py, pz) = p in
   M.lemma_div_mod_prime_is_zero #prime px pz;
   M.lemma_div_mod_prime_is_zero #prime py pz
@@ -22,7 +25,7 @@ let aff_point_add_assoc_lemma p q s = admit ()
 
 let aff_point_add_comm_lemma p q = admit()
 
-let to_aff_point_at_infinity_lemma () = admit()
+let to_aff_point_at_infinity_lemma #c = admit()
 
 let to_aff_point_add_lemma p q = admit()
 
