specs/lemmas/Spec.P256.Lemmas.fsti
@@ -12,32 +12,41 @@ open Spec.P256.PointOps
 
 // TODO: add `point_inv p = is_on_curve p || is_point_at_inf p`
 
-val prime_lemma: unit -> Lemma (FStar.Math.Euclid.is_prime prime)
+val prime_lemma: c:curve_params ->
+    Lemma (FStar.Math.Euclid.is_prime c.prime /\
+           FStar.Math.Euclid.is_prime c.order)
 
-val lemma_aff_is_point_at_inf: p:proj_point ->
+val lemma_exp_prime: p:nat{FStar.Math.Euclid.is_prime p} -> x:nat{x < p} ->
+  Lemma (Lib.NatMod.pow_mod #p x (p-1) == 1)
+
+val lemma_exp_inv_prime: p:nat{FStar.Math.Euclid.is_prime p} ->
+  x:nat{x < p} -> y:nat ->
+  Lemma (x * y % p == 1 ==> Lib.NatMod.pow_mod #p x (p-2) == y % p)
+
+val lemma_aff_is_point_at_inf: {| curve_params |} -> p:proj_point ->
   Lemma (let px, py, pz = p in
     is_aff_point_at_inf (to_aff_point p) == (pz = 0 || (px = 0 && py = 0)))
 
 
-val aff_point_at_inf_lemma (p:aff_point) :
+val aff_point_at_inf_lemma {| curve_params |}  (p:aff_point) :
   Lemma (aff_point_add p aff_point_at_inf = p)
 
 
-val aff_point_add_assoc_lemma (p q s:aff_point) :
+val aff_point_add_assoc_lemma {| curve_params |} (p q s:aff_point) :
   Lemma (aff_point_add (aff_point_add p q) s == aff_point_add p (aff_point_add q s))
 
 
-val aff_point_add_comm_lemma (p q:aff_point) :
+val aff_point_add_comm_lemma {| curve_params |} (p q:aff_point) :
   Lemma (aff_point_add p q = aff_point_add q p)
 
 
-val to_aff_point_at_infinity_lemma: unit ->
+val to_aff_point_at_infinity_lemma {| curve_params |} :
   Lemma (to_aff_point point_at_inf == aff_point_at_inf)
 
 
-val to_aff_point_add_lemma (p q:proj_point) :
+val to_aff_point_add_lemma {| curve_params |} (p q:proj_point) :
   Lemma (to_aff_point (point_add p q) == aff_point_add (to_aff_point p) (to_aff_point q))
 
 
-val to_aff_point_double_lemma (p:proj_point) :
+val to_aff_point_double_lemma {| curve_params |} (p:proj_point) :
   Lemma (to_aff_point (point_double p) == aff_point_add (to_aff_point p) (to_aff_point p))
